generational/spec/GC.Gen.CheneyGraphReadiness.fst
@@ -4023,6 +4023,10 @@ let chunked_cheney_collect_then_major_gc_live_subgraph_from_pre_promote_nonblue_
       SpecMajorAlloc.major_fl_chain_terminates major fp alloc_fuel = true /\
       GenInv.chunked_chain_objects_blue major fp alloc_fuel /\
       chunked_minor_preflight_value_policy minor major fp roots fresh /\
+      CInj.chunked_minor_major_fields_nonblue_non_infix_targets minor major /\
+      (SpecMajorAlloc.major_fl_head_wosize major fp <
+       PromotionDemand.minor_promotion_demand minor + 1 ==>
+       CInj.chunked_minor_fields_miss_chunk minor fresh) /\
       (let r =
        SpecMajorAlloc.ensure_major_head_capacity_spec
         major fp alloc_fuel
@@ -4048,8 +4052,6 @@ let chunked_cheney_collect_then_major_gc_live_subgraph_from_pre_promote_nonblue_
        (forall (target: obj_addr).
         Seq.mem target (MH.major_objects r.capacity_major_out) ==>
         Fields.is_pointer_field target) /\
-       CInj.chunked_minor_major_fields_nonblue_non_infix_targets
-        minor r.capacity_major_out /\
        CheneyPres.chunked_cheney_promote_split_ready
         minor r.capacity_major_out r.capacity_fp_out roots
         r.capacity_fuel_out /\
@@ -4110,6 +4112,12 @@ let chunked_cheney_collect_then_major_gc_live_subgraph_from_pre_promote_nonblue_
             minor r.capacity_major_out);
   assert (GenInv.chunked_major_alloc_shape
             r.capacity_major_out r.capacity_fp_out r.capacity_fuel_out);
+  assert (SpecMajorAlloc.major_fl_head_wosize major fp < needed ==>
+          MH.chunk_disjoint_from_all fresh major);
+  CInj.chunked_minor_major_fields_nonblue_non_infix_targets_ensure_head_capacity
+    minor major fp alloc_fuel needed fresh;
+  assert (CInj.chunked_minor_major_fields_nonblue_non_infix_targets
+            minor r.capacity_major_out);
   assert (SpecMajorAlloc.major_fl_chain_terminates
             r.capacity_major_out r.capacity_fp_out r.capacity_fuel_out = true);
   assert (GenInv.chunked_chain_objects_blue
